theories/FOL/ModelTheory/AnalysisLS.v
@@ -1,0 +1,42 @@
+Require Import Undecidability.FOL.ModelTheory.LogicalPrinciples.
+Require Import Undecidability.FOL.ModelTheory.HenkinEnv.
+Require Import Undecidability.FOL.ModelTheory.ReverseLS. 
+Require Import Undecidability.FOL.ModelTheory.Core.
+
+Section LSiffDC.
+
+    Corollary LS_iff_DC_under_AC00_LEM: 
+        AC00 -> LEM -> LS <-> DC.
+    Proof.
+        intros H1 H2; split.
+        - eapply LS_CC_impl_DC; eauto.
+        - intros DC. eapply LS_downward_with_DC_LEM; eauto.
+    Qed.
+
+    Corollary LS_iff_DC_BDP_BEP_under_AC00:
+        AC00 -> LS <-> DC /\ BDP /\ BEP.
+    Proof.
+        intros H1; split.
+        - intros HLS. repeat split.
+          now apply LS_CC_impl_DC.
+          now apply LS_impl_BDP.
+          now apply LS_impl_BEP.
+        - intros (h1 & h2 & h3).
+          now apply LS_downward_with_BDP_BEP_DC.
+    Qed.
+
+    Corollary LS_iff_DDC_BDP_BEP_BCC:
+        LS <-> DDC /\ BDP /\ BEP /\ BCC.
+    Proof.
+        split.
+        - intros HLS. repeat split.
+          assert (OBDC) as HO. now  apply LS_impl_OBDC.
+          assert (BDC2) as H2. intros X. now apply OBDC_impl_BDC2_on.
+          now apply BDC2_iff_DDC_BCC.
+          now apply LS_impl_BDP. now apply LS_impl_BEP.
+          now apply LS_impl_BCC.
+        - intros (h1 & h2 & h3 & h4).
+          now apply LS_downward.
+    Qed.
+
+End LSiffDC.
